\chapter{Detailed Calculation of Two coupled Two-level systems\label{app:chap3_appendix}}
For $\oper{H}_{\mathrm{S}}=0$, the global Hamiltonian reads
\begin{equation}
\oper{H}=\underbrace{\oper{\sigma}_{\mathrm{C}, x}}_{=1_S \otimes \oper{H}_{\mathrm{C}}}+\underbrace{\left(\oper{\sigma}_{\mathrm{S}, x}+\oper{\sigma}_{\mathrm{S}, x}\right) \otimes \oper{\sigma}_{\mathrm{C}, x}}_{=\oper{V}}=\left(\begin{array}{cccc}
1 & 1 & 0 & 1 \\
1 & -1 & 1 & 0 \\
0 & 1 & 1 & -1 \\
1 & 0 & -1 & -1
\end{array}\right)
\end{equation}
and has eigenvalues
\(E=\{-\sqrt{3}, \sqrt{3}\}\), 
both with multiplicity two. The Eigenvectors corresponding to them are
\begin{equation}
\begin{pmatrix}
1 \\
0 \\
-1 \\
-(1+\sqrt{3})
\end{pmatrix},\begin{pmatrix}
0 \\
1 \\
1-\sqrt{3} \\
-1
\end{pmatrix},\begin{pmatrix}
1 \\
0 \\
-1 \\
\sqrt{3}-1
\end{pmatrix},\begin{pmatrix}
0 \\
1 \\
1+\sqrt{3} \\
-1
\end{pmatrix}
\end{equation}
for components $\left\{\left|\uparrow_S \uparrow_C
\right\rangle,\left|\uparrow_S \downarrow_C\right\rangle,
\left|\downarrow_S \uparrow_C\right\rangle,\left|\downarrow_S 
\downarrow_C\right\rangle\right\}$. 

One can check for $|\Psi\rangle=\left|\uparrow_S \uparrow_{\mathrm{C}}\right\rangle
-\left|\downarrow_{\mathrm{S}} \uparrow_{\mathrm{C}}\right\rangle-(1+\sqrt{3})\left|
\downarrow_{\mathrm{s}} \downarrow_{\mathrm{C}}\right\rangle$, 
which we have takes as the global state in \refsec{sec:chap3_2spin_interact}, yields
\begin{equation}
\begin{aligned}
\oper{H}|\Psi\rangle= & \left(\left|\uparrow_{\mathrm{s}} \uparrow_{\mathrm{C}}\right\rangle+\left|\uparrow_{\mathrm{s}} \downarrow_{\mathrm{C}}\right\rangle+\left|\downarrow_{\mathrm{s}} \downarrow_{\mathrm{C}}\right\rangle\right) \\
& -\left(\left|\downarrow_{\mathrm{s}} \uparrow_{\mathrm{C}}\right\rangle+\left|\uparrow_{\mathrm{s}} \downarrow_{\mathrm{C}}\right\rangle-\left|\downarrow_{\mathrm{s}} \downarrow_{\mathrm{C}}\right\rangle\right) \\
& -(\sqrt{3}+1)\left(-\left|\downarrow_{\mathrm{S}} \downarrow_{\mathrm{C}}\right\rangle+\left|\uparrow_{\mathrm{s}} \uparrow_{\mathrm{C}}\right\rangle-\left|\downarrow_{\mathrm{s}} \uparrow_{\mathrm{C}}\right\rangle\right) \\
= & -\sqrt{3}\left|\uparrow_{\mathrm{s}} \uparrow_{\mathrm{C}}\right\rangle+\sqrt{3}\left|\downarrow_{\mathrm{s}} \uparrow_{\mathrm{C}}\right\rangle+(\sqrt{3}+3)\left|\downarrow_{\mathrm{s}} \downarrow_{\mathrm{C}}\right\rangle \\
= & -\sqrt{3}|\Psi\rangle .
\end{aligned}
\end{equation}

We define $c \equiv 1+\sqrt{3}$ and take the clock state to be
\begin{equation}
|\chi(\lambda)\rangle_{\mathrm{C}}=e^{i E \lambda}\left[a_0 e^{-i g \lambda}\left|\uparrow_{\mathrm{C}}\right\rangle_{\mathrm{C}}+a_1 e^{i g \lambda}\left|\downarrow_{\mathrm{C}}\right\rangle_{\mathrm{C}}\right]
\end{equation}

Then, the unnormalized system state becomes
\begin{equation}
\begin{aligned}
|\phi\rangle_{\mathrm{S}}= & \langle\chi(\lambda) \mid \Psi\rangle_{\mathrm{C}} \\
= & e^{-i E \lambda}\left[a_0^* e^{i g \lambda}\left|\uparrow_{\mathrm{S}}\right\rangle_{\mathrm{S}} 
-\left(c a_1^* e^{-i g \lambda}+a_0^* e^{i g \lambda}\right)\left|\downarrow_{\mathrm{S}}\right\rangle_{\mathrm{S}}\right] .
\end{aligned}
\end{equation}

For simplicity, we use $a_0=a_1=1$ with $\langle\chi \mid \chi\rangle_{\mathrm{C}}=2$. The $\lambda$-dependent unnormalized state is
\begin{equation}
\begin{aligned}
|\phi(\lambda)\rangle_{\mathrm{S}} & =\langle\chi(\lambda) \mid \Psi\rangle_{\mathrm{C}} \\
& =e^{i \sqrt{3} \lambda}\left[e^{i \lambda}\left|\uparrow_{\mathrm{S}}\right\rangle_{\mathrm{S}}-\left(c e^{-i \lambda}+e^{i \lambda}\right)\left|\downarrow_{\mathrm{S}}\right\rangle_{\mathrm{S}}\right] \\
& =e^{i c \lambda}\left[\left|\uparrow_{\mathrm{S}}\right\rangle_{\mathrm{S}}-\left(c e^{-2 i \lambda}+1\right)\left|\downarrow_{\mathrm{S}}\right\rangle_{\mathrm{S}}\right]
\end{aligned}
\end{equation}
with norm
\begin{equation}
\begin{aligned}
\langle\phi \mid \phi\rangle_{\mathrm{S}} & =\left\langle\uparrow_{\mathrm{S}} \mid \uparrow_{\mathrm{S}}\right\rangle_{\mathrm{S}}+\left|c+e^{2 i \lambda}\right|^2\left\langle\downarrow_{\mathrm{S}} \mid \downarrow_{\mathrm{S}}\right\rangle_{\mathrm{S}} \\
& =1+\underbrace{c^2}_{=2(2+\sqrt{3})}+1+c \underbrace{\left(e^{2 i \lambda}+e^{-2 i \lambda}\right)}_{=2 \cos (2 \lambda)} \\
& =2[3+\sqrt{3}+c \cos (2 \lambda)] \\
& =2[2+c(1+\cos (2 \lambda))] \\
& =4\left[1+c \cos ^2(\lambda)\right]
\end{aligned}
\end{equation}
and
\begin{equation}
\sqrt{\langle\phi \mid \phi\rangle_{\mathrm{S}}}=2 \sqrt{1+c \cos ^2(\lambda)} .
\end{equation}

For $\lambda=0$. the initial state reads
\begin{equation}
|\phi(0)\rangle_{\mathrm{S}}=\left|\uparrow_{\mathrm{S}}\right\rangle_{\mathrm{S}}-(\sqrt{3}+2)\left|\downarrow_{\mathrm{S}}\right\rangle_{\mathrm{S}} .
\end{equation}

With the expression
\begin{equation}
\begin{aligned}
\oper{V}|\Psi\rangle= & \left(\left|\downarrow_S \downarrow_C\right\rangle+\left|\uparrow_S \downarrow_C\right\rangle\right)-\left(\left|\uparrow_S \downarrow_C\right\rangle-\left|\downarrow_S \downarrow_C\right\rangle\right) \\
& -c\left(\left|\uparrow_s \uparrow_C\right\rangle-\left|\downarrow_s \uparrow_C\right\rangle\right) \\
= & -c\left|\uparrow_s \uparrow_C\right\rangle+c\left|\downarrow_s \uparrow_C\right\rangle+2\left|\downarrow_S \downarrow_C\right\rangle,
\end{aligned}
\end{equation}
we determine
\begin{equation}
\begin{aligned}
\langle\chi(\lambda)|\oper{V}| \Psi\rangle_{\mathrm{C}}= & e^{-i E \lambda}\left[-c e^{i \lambda}\left|\uparrow_{\mathrm{S}}\right\rangle_{\mathrm{S}}+c e^{i \lambda}\left|\downarrow_{\mathrm{S}}\right\rangle_{\mathrm{S}}\right. \\
& \left.+2 e^{-i \lambda}\left|\downarrow_{\mathrm{S}}\right\rangle_{\mathrm{S}}\right] \\
= & e^{-i E \lambda}\left[-c e^{i \lambda}\left|\uparrow_{\mathrm{S}}\right\rangle_{\mathrm{S}}+\left(c e^{i \lambda}+2 e^{-i \lambda}\right)\left|\downarrow_{\mathrm{S}}\right\rangle_{\mathrm{S}}\right] \\
= & e^{-i E \lambda} e^{i \lambda}\left[-c\left|\uparrow_{\mathrm{S}}\right\rangle_{\mathrm{S}}+\left(c+2 e^{-2 i \lambda}\right)\left|\downarrow_{\mathrm{S}}\right\rangle_{\mathrm{S}}\right]
\end{aligned}
\end{equation}

Using also
\begin{equation}
\left\langle\left.\phi\right|_{\mathrm{S}}=e^{i E \lambda} e^{-i \lambda}\left[\left|\uparrow_{\mathrm{S}}\right\rangle_{\mathrm{S}}-\left(c e^{2 i \lambda}+1\right)\left|\downarrow_{\mathrm{S}}\right\rangle_{\mathrm{S}}\right],\right.
\end{equation}
allows us to express
\begin{equation}
\begin{aligned}
\left\langle\chi\left|\oper{V} \oper{P}_{\Psi}\right| \chi\right\rangle_{\mathrm{C}}= & {\left[-c\left|\uparrow_{\mathrm{s}}\right\rangle_{\mathrm{s}}+\left(c+2 e^{-2 i \lambda}\right)\left|\downarrow_{\mathrm{s}}\right\rangle_{\mathrm{s}}\right] } \\
& \otimes\left[\left\langle\left.\uparrow_{\mathrm{s}}\right|_{\mathrm{s}}-\left(c e^{2 i \lambda}+1\right)\left\langle\left.\downarrow_{\mathrm{s}}\right|_{\mathrm{s}}\right]\right.\right. \\
= & -\left.c\left|\uparrow_{\mathrm{s}}\right\rangle \uparrow_{\mathrm{s}}\right|_{\mathrm{s}}+c\left(c e^{2 i \lambda}+1\right)\left|\uparrow_{\mathrm{s}}\right\rangle\left\langle\left.\downarrow_{\mathrm{s}}\right|_{\mathrm{s}}\right. \\
& +\left.\left(c+2 e^{-2 i \lambda}\right)\left|\downarrow_{\mathrm{S}}\right\rangle \uparrow_{\mathrm{s}}\right|_{\mathrm{s}} \\
& -\left.\left(c e^{2 i \lambda}+1\right)\left(c+2 e^{-2 i \lambda}\right)\left|\downarrow_{\mathrm{S}}\right\rangle \downarrow_{\mathrm{S}}\right|_{\mathrm{s}}
\end{aligned}
\end{equation}

and
\begin{equation}
\begin{aligned}
& \left\langle\chi\left|\oper{P}_W \oper{V}\right| \chi\right\rangle_{\mathrm{C}}=-c\left|\uparrow_{\mathrm{S}}\right\rangle\left\langle\left.\uparrow_{\mathrm{S}}\right|_{\mathrm{S}}+c\left(c e^{-2 i \lambda}+1\right) \mid \downarrow_{\mathrm{S}}\right\rangle\left\langle\left.\uparrow_{\mathrm{S}}\right|_{\mathrm{S}}\right. \\
& +\left(c+2 e^{2 i \lambda}\right)\left|\uparrow_s\right\rangle\left\langle\left.\downarrow_s\right|_s\right. \\
& -\left(c e^{-2 i \lambda}+1\right)\left(c+2 e^{2 i \lambda}\right)\left|\downarrow_S K \downarrow_S\right|_s \\
&
\end{aligned}
\end{equation}

With the definition
\begin{equation}
f(\lambda)=\cos (2 \lambda)+c \cos ^2(\lambda),
\end{equation}
the individual components read
\begin{equation}
\begin{aligned}
\left\langle\uparrow_{\mathrm{S}} \chi\left|\left\{\oper{P}_{\Psi}, \oper{V}\right\}\right| \uparrow_{\mathrm{S}} \chi\right\rangle_{\mathrm{C}} & =-2 c \\
\left\langle\uparrow_{\mathrm{S}} \chi\left|\left\{\oper{P}_{\Psi}, \oper{V}\right\}\right| \downarrow_{\mathrm{S}} \chi\right\rangle_{\mathrm{C}} & =c\left(c e^{2 i \lambda}+1\right)+\left(c+2 e^{2 i \lambda}\right) \\
& =2\left[2 \cos (2 \lambda)+c\left(1+e^{2 i \lambda}\right)\right] \\
& =4\left[\cos (2 \lambda)+c \cos ^2(\lambda)\right]+2 i c \sin (2 \lambda) \\
& =4 f(\lambda)+2 i c \sin (2 \lambda)
\end{aligned}
\end{equation}
$\left\langle\downarrow_{\mathrm{s}} \chi\left|\left\{\oper{P}_{\Psi}, \oper{V}\right\}\right| \uparrow_{\mathrm{s}} \chi\right\rangle_{\mathrm{C}}=4\left[\cos (2 \lambda)+c \cos ^2(\lambda)\right]-2 i c \sin (2 \lambda) \quad$ and
\begin{equation}
=4 f(\lambda)-2 i c \sin (2 \lambda)
\end{equation}
\begin{equation}
\left\langle\downarrow_{\mathrm{s}} \chi\left|\left\{\oper{P}_{\Psi}, \oper{V}\right\}\right| \downarrow_{\mathrm{s}} \chi\right\rangle_{\mathrm{C}}=-2 \operatorname{Re}\left(c e^{2 i \lambda}+1\right) \cdot\left(c+2 e^{-2 i \lambda}\right)
\end{equation}
\begin{equation}
=-2 \operatorname{Re}\left[2\left(e^{2 i \lambda}+e^{-2 i \lambda}\right)+2 c\left(1+e^{2 i \lambda}\right)+c\right]
\end{equation}
\begin{equation}
=-2[4 \cos (2 \lambda)+2 c(1+\cos (2 \lambda))+c]
\end{equation}
\begin{equation}
=-2\left[4 \cos (2 \lambda)+4 c \cos ^2(\lambda)+c\right]
\end{equation}
\begin{equation}
\begin{aligned}
& =-8\left[\cos (2 \lambda)+c \cos ^2(\lambda)\right]-2 c \\
& =-8 f(\lambda)-2 c .
\end{aligned}
\end{equation}

Thus, the main part of the effective system potential is
\begin{equation}
\begin{aligned}
\left\langle\chi\left|\left\{\oper{V}, \oper{P}_\psi\right\}\right| \chi\right\rangle_{\mathrm{C}}= & -2 c \sin (2 \lambda) \oper{\sigma}_{\mathrm{s}, y}+4 f(\lambda)\left(\oper{\sigma}_{\mathrm{S}, x}+\oper{\sigma}_{\mathrm{S}, x}\right) \\
& -2[c+2 f(\lambda)] \mathrm{i}_{\mathrm{S}} .
\end{aligned}
\end{equation}
in terms of Pauli operators. In addition,
\begin{equation}
\begin{aligned}
\left\langle\Psi\left|\oper{V} \oper{P}_\chi\right| \Psi\right\rangle= & {\left[-c\left\langle\left.\uparrow_{\mathrm{S}}\right|_{\mathrm{S}}+\left(c+2 e^{2 i \lambda}\right)\left\langle\left.\downarrow_{\mathrm{S}}\right|_{\mathrm{S}}\right]\right.\right.} \\
& \cdot\left[\left|\uparrow_{\mathrm{S}}\right\rangle_{\mathrm{S}}-\left(c e^{-2 i \lambda}+1\right)\left|\downarrow_{\mathrm{S}}\right\rangle_{\mathrm{S}}\right] \\
& =-c-\left(c+2 e^{2 i \lambda}\right)\left(c e^{-2 i \lambda}+1\right) \\
& =-[2 c+2 e^{2 i \lambda}+\underbrace{c^2}_{=2(1+c)} e^{-2 i \lambda}+2 c] \\
= & -2\left[2 c+e^{2 i \lambda}+(1+c) e^{-2 i \lambda}\right] \\
= & -2\left[2 c+e^{2 i \lambda}+e^{-2 i \lambda}+c e^{-2 i \lambda}\right] \\
= & -2[2 c+2 \cos (2 \lambda)+c \cos (2 \lambda)-i \sin (2 \lambda)] \\
= & 2 i \sin (2 \lambda)-2[2 c+(2+c) \cos (2 \lambda)] \\
= & 2 i \sin (2 \lambda)-2\left[2 c+(2+c)\left(2 \cos ^2(\lambda)-1\right)\right]
\end{aligned}
\end{equation}
\begin{equation}
\begin{aligned}
\operatorname{Re}\left\langle\Psi\left|\oper{V} \oper{P}_\chi\right| \Psi\right\rangle & =-2[2 c+(2+c) \cos (2 \lambda)] \\
& =-2\left[c+2\left(\cos (2 \lambda)+c \cos ^2(\lambda)\right)\right] \\
& =-2[c+2 f(\lambda)]
\end{aligned}
\end{equation}

Hence,
and
\begin{equation}
\oper{V}_{\mathrm{S}}=\frac{\left\langle\chi\left|\left\{\oper{V}, \oper{P}_{\Psi}\right\}\right| \chi\right\rangle_{\mathrm{C}}-\operatorname{Re}\left\langle\Psi\left|\oper{V} \oper{P}_\chi\right| \Psi\right\rangle \oper{1}_{\mathrm{S}}}{\left\langle\Psi\left|\oper{P}_\chi\right| \Psi\right\rangle}
\end{equation}
\begin{equation}
=\frac{-c \sin (2 \lambda)}{2\left[1+c \cos ^2(\lambda)\right]} \oper{\sigma}_{\mathrm{S}, y}+\frac{\cos (2 \lambda)+c \cos ^2(\lambda)}{\left[1+c \cos ^2(\lambda)\right]}\left(\oper{\sigma}_{\mathrm{S}, x}+\oper{\sigma}_{\mathrm{S}, z}\right)
\end{equation}
\begin{equation}
\equiv \vec{V}_s(\lambda) \cdot \oper{\sigma}
\end{equation}
